use intro tag to track Introed EX vars, generate annotation for code after loop

annotated/annotation_proofauto.v
@@ -1,6 +1,8 @@
 Require Export VST.floyd.proofauto.
 Require Export annotated_Clight.
 
+(********** annotation handling lemmas ****************************************)
+
 Lemma decorate_C_skip: forall P,
   P ->
   let d := @abbreviate _ Sskip in P.
@@ -108,11 +110,33 @@ Proof.
   exact H.
 Qed.
 
+Ltac fill_decorate_C_loop_after d :=
+  match d with
+  | Ssequence Sbreak ?d2 => refine d2
+  | Ssequence ?d1 ?d2 =>
+      first [fill_decorate_C_loop_after d1 | fill_decorate_C_loop_after d2]
+  | Sgiven ?A ?d1 =>
+    match d1 with
+    | (fun x => _) =>
+        refine (Sgiven A _); first [intro x | let x1 := fresh x in rename x into x1; intro x];
+        let d2 := eval cbv beta in (d1 x) in fill_decorate_C_loop_after d2
+    end
+  | Sifthenelse _ ?d1 ?d2 =>
+      first [fill_decorate_C_loop_after d1 | fill_decorate_C_loop_after d2]
+  | _ => fail
+  end.
+
+Ltac fill_decorate_C_loop_after2 :=
+  match goal with
+  | d := @abbreviate _ (Ssequence (Sloop _ ?d1 ?d2) _) |- _ =>
+      fill_decorate_C_loop_after d1
+  end.
+
 Lemma decorate_C_loop_after:
   forall {Espec: OracleKind} {cs: compspecs},
-    forall d1 Inv d2 d3 Delta P c Post,
-      (let d := @abbreviate _ d3 in semax Delta P c Post) ->
-      (let d := @abbreviate _ (Ssequence (Sloop Inv d1 d2) d3) in semax Delta P c Post).
+    forall (d1 d2: statement) Delta P c Post,
+      (let d := @abbreviate _ d1 in semax Delta P c Post) ->
+      (let d := @abbreviate _ d2 in semax Delta P c Post).
 Proof.
   intros.
   exact H.
@@ -120,28 +144,27 @@ Qed.
 
 Lemma decorate_C_step2:
   forall {Espec: OracleKind} {cs: compspecs},
-    forall d1 d2 Delta P c Post,
+    forall d1 d2 P,
       (* should check d1 not Sassert or Sassume *)
-      (let d := @abbreviate _ d2 in semax Delta P c Post) ->
-      (let d := @abbreviate _ (Ssequence d1 d2) in semax Delta P c Post).
+      (let d := @abbreviate _ d2 in P) ->
+      (let d := @abbreviate _ (Ssequence d1 d2) in P).
 Proof.
   intros.
-  exact H.
+  assumption.
 Qed.
 
 Lemma decorate_C_step1:
   forall {Espec: OracleKind} {cs: compspecs},
-    forall (d1: statement) Delta P c Post,
+    forall (d1: statement) P,
       (* should check d1 not Sassert or Sassume *)
-      semax Delta P c Post ->
-      (let d := @abbreviate _ d1 in semax Delta P c Post).
+      P ->
+      (let d := @abbreviate _ d1 in P).
 Proof.
   intros.
-  exact H.
+  assumption.
 Qed.
 
-
-
+(*
 Lemma decorate_C_if_then1:
   forall {Espec: OracleKind} {cs: compspecs},
     forall b d1 d2 Delta P c Post,
@@ -181,7 +204,9 @@ Proof.
   intros.
   exact H.
 Qed.
+*)
 
+(*
 Lemma decorate_C_while_body2:
   forall {Espec: OracleKind} {cs: compspecs},
     forall b d1 Inv d2 Delta P c Post,
@@ -201,6 +226,7 @@ Proof.
   intros.
   exact H.
 Qed.
+*)
 
 (* Lemma decorate_C_assert:
   forall {Espec: OracleKind} {cs: compspecs},
@@ -228,40 +254,54 @@ Proof.
   + exact H0.
 Qed. *)
 
+Definition Intros_tag {A} (x : A) := True.
 
 Lemma decorate_C_given:
   forall {Espec: OracleKind} {cs: compspecs},
     forall {A: Type} d1 Delta P c Post,
-      (forall a, let d := @abbreviate _ (d1 a) in semax Delta (P a) c Post) ->
+      (forall a, Intros_tag a -> let d := @abbreviate _ (d1 a) in semax Delta (P a) c Post) ->
       (let d := @abbreviate _ (Sgiven A d1) in semax Delta (exp P) c Post).
 Proof.
   intros.
   Intros a.
-  apply H.
+  apply H. apply I.
 Qed.
 
 Lemma decorate_C_given':
   forall {Espec: OracleKind} {cs: compspecs},
     forall {A: Type} a d1 Delta P c Post,
-      (let d := @abbreviate _ (d1 a) in semax Delta P c Post) ->
+      (Intros_tag a -> let d := @abbreviate _ (d1 a) in semax Delta P c Post) ->
       (let d := @abbreviate _ (Sgiven A d1) in semax Delta P c Post).
 Proof.
   intros.
-  apply H.
+  apply H. apply I.
 Qed.
 
+Lemma delta_derives_refl:
+  forall Delta P,
+    ENTAIL Delta, P |-- P.
+Proof.
+  intros. apply andp_left2. apply derives_refl.
+Qed.
 
 Tactic Notation "forwardD" :=
   lazymatch goal with
+  (* entailment *)
+  | |- let d := @abbreviate _ _ in ENTAIL _, _ |-- _ =>
+      intro d; clear d
+  (* skip *)
   | |- let d := @abbreviate _ Sskip in _ =>
       refine (decorate_C_skip _ _)
+  (* dummyassert *)
   | |- let d := @abbreviate _ (Ssequence (Sdummyassert _) _) in _ =>
       refine (decorate_C_dummyassert _ _ _ _)
+  (* assert as postcondition *)
   | |- let d := @abbreviate _ (Ssequence _ (Ssequence (Sassert ?P) _)) in _ => 
       refine (decorate_C_assert2 _ _ _ _ _ _ _ _ _ _);
       [ intro d; abbreviate_semax; revert d
       | intro d; abbreviate_semax; revert d
       ]
+  (* if *)
   | |- let d := @abbreviate _ (Ssequence (Sifthenelse _ _ _) _) in
        (* semax _ _ (Clight.Sifthenelse _ _ _) _ => *)
        _ =>
@@ -269,6 +309,7 @@ Tactic Notation "forwardD" :=
       [ ..
       | revert d; refine (decorate_C_if_then _ _ _ _ _ _ _ _ _)
       | revert d; refine (decorate_C_if_else _ _ _ _ _ _ _ _ _)]
+  (* while *)
   | |- let d := @abbreviate _ (Ssequence (Swhile ?Inv _ _) _) in
        (* semax _ _ (Clight.Ssequence (Clight.Swhile _ _) _) _ => *)
        _ =>
@@ -276,26 +317,51 @@ Tactic Notation "forwardD" :=
       [ ..
       | revert d; refine (decorate_C_while_body _ _ _ _ _ _ _ _ _)
       | revert d; refine (decorate_C_while_after _ _ _ _ _ _ _ _ _)]
+  (* loop single inv *)
   | |- let d := @abbreviate _ (Ssequence (Sloop (LISingle ?Inv) _ _) _) in
-       (* semax _ _ (Clight.Ssequence (Clight.Sloop _ _) _) _ => *)
-       _ =>
+       semax _ _ (Clight.Sloop _ _) _ =>
       intro d; forward_loop Inv;
       [ ..
       | revert d; refine (decorate_C_loop_body _ _ _ _ _ _ _ _ _)]
+  (* loop double inv *)
   | |- let d := @abbreviate _ (Ssequence (Sloop (LIDouble ?Inv1 ?Inv2) _ _) _) in
-       (* semax _ _ (Clight.Ssequence (Clight.Sloop _ _) _) _ => *)
-       _ =>
+       semax _ _ (Clight.Sloop _ _) _ =>
       intro d; forward_loop Inv1 continue: Inv2;
       [ ..
       | revert d; refine (decorate_C_loop_body _ _ _ _ _ _ _ _ _)
       | revert d; refine (decorate_C_loop_incr _ _ _ _ _ _ _ _ _)]
+  (* loop single inv without postcondition *)
+  | |- let d := @abbreviate _ (Ssequence (Sloop (LISingle ?Inv) _ _) _) in
+       (* semax _ _ (Clight.Ssequence (Clight.Sloop _ _) _) _ => *)
+       _ =>
+      let Post := fresh "Post" in
+      evar (Post : assert);
+      intro d;
+      set (d1 := ltac: (fill_decorate_C_loop_after2));
+      forward_loop Inv break: Post;
+      [ ..
+      | revert d; refine (decorate_C_loop_body _ _ _ _ _ _ _ _ _)
+      | revert d; refine (decorate_C_loop_after d1 _ _ _ _ _ _)]
+  (* loop double inv without postcondition*)
+  | |- let d := @abbreviate _ (Ssequence (Sloop (LIDouble ?Inv1 ?Inv2) _ _) _) in
+       (* semax _ _ (Clight.Ssequence (Clight.Sloop _ _) _) _ => *)
+       _ =>
+      let Post := fresh "Post" in
+      evar (Post : assert);
+      set (d1 := ltac: (fill_decorate_C_loop_after2));
+      intro d; forward_loop Inv1 continue: Inv2 break: Post;
+      [ ..
+      | revert d; refine (decorate_C_loop_body _ _ _ _ _ _ _ _ _)
+      | revert d; refine (decorate_C_loop_incr _ _ _ _ _ _ _ _ _)
+      | revert d; refine (decorate_C_loop_after d1 _ _ _ _ _ _)]
+  (* given *)
   | |- let d := @abbreviate _ (Sgiven _ (fun x => _)) in
        semax _ _ _ _ =>
       refine (decorate_C_given _ _ _ _ _ _);
       first
       [ intro x
       | let old_x := fresh x in rename x into old_x; intro x];
-      intro d; Intros; revert d
+      intros ? d; Intros; revert d
       ;try match goal with
       | |- let d := @abbreviate _ (Ssequence (Sdummyassert _) _) in _ =>
       refine (decorate_C_dummyassert _ _ _ _)
@@ -308,10 +374,10 @@ Tactic Notation "forwardD" :=
       intro d;
       forward;
       revert d;
-      refine (decorate_C_step2 _ _ _ _ _ _ _)
+      refine (decorate_C_step2 _ _ _ _)
   | |- let d := @abbreviate _ _ in
        semax _ _ _ _ =>
-      refine (decorate_C_step1 _ _ _ _ _ _);
+      refine (decorate_C_step1 _ _ _);
       forward
   end.
 
@@ -319,5 +385,5 @@ Tactic Notation "forwardD" constr(a) :=
   match goal with
   | |- let d := @abbreviate _ (Sgiven _ (fun x => _)) in
        semax _ _ _ _ =>
-      refine (decorate_C_given' a _ _ _ _ _ _); intros d; Intros; revert d
+      refine (decorate_C_given' a _ _ _ _ _ _); intros ? d; Intros; revert d
   end.
