annotated/append_verif.v
@@ -32,6 +32,7 @@ match goal with
 | |- ?P => let d1 := eval hnf in f_append_hint in
            change (let d := @abbreviate _ d1 in P)
 end.
+cbv delta [Swhile].
 forwardD sh.
 forwardD s1.
 forwardD s2.
@@ -61,17 +62,20 @@ forwardD.
   forwardD.
   forwardD.
   forwardD.
-  forwardD.
   {
     Exists a s1b x u.
     subst s1. entailer!. simpl. cancel_wand.
   }
   {
+    (* clear a s1b H0 u. *) (* Without clearing deadvars here, we will have "a is already used later" *)
+    (* Intro EXs *)
     forwardD.
     forwardD.
     forwardD.
     forwardD.
+    (* forward_if *)
     forwardD.
+    (* then branch *)
     forwardD.
     {
       destruct s1b as [| b s1c]; unfold listrep at 3; fold listrep; [ Intros; contradiction |].
@@ -95,22 +99,29 @@ forwardD.
       forget (b::s1c++s2) as s3.
       unfold listrep; fold listrep; Exists u; auto.
     }
+    (* else branch *)
+    forwardD.
     forwardD.
     {
-      Exists a t u. entailer!. rewrite (proj1 H4 (eq_refl _)). simpl. cancel.
+      unfold Post. Exists a s1b t u H13. apply delta_derives_refl.
+      (*  entailer!. rewrite (proj1 H4 (eq_refl _)). simpl. cancel. *)
     }
   }
   {
+    cbv delta [Post d1].
     forwardD.
     forwardD.
     forwardD.
+    forwardD.
+    intro d; Intro H13; revert d.
     forwardD.
     forwardD.
     {
       Exists x.
       entailer!.
+      rewrite (proj1 H16 (eq_refl _)). simpl.
       unfold listrep at 3; fold listrep. normalize.
-      pull_right (listrep sh (a :: s2) t -* listrep sh ((a0 :: s1b) ++ s2) x).
+      pull_right (listrep sh (a :: s2) t -* listrep sh ((a0 :: s1b0) ++ s2) x).
       apply modus_ponens_wand'.
       unfold listrep at 2; fold listrep. Exists y; auto.
     }
